coq/NNRSimp/Optim/TNNRSimpUnflatten.v
@@ -55,602 +55,602 @@ Section TNNRSimpUnflatten.
           forall τ,
             [ Γc ; Γ  ⊢ e ▷ Coll (Coll τ) ] ->
             forall d d',
-            lookup equiv_dec σ v = Some d ->
-        lift2P flattens_to d d' ->
-        lift2P
-          flattens_to
-          (nnrs_imp_expr_eval brand_relation_brands σc σ e)
-          (nnrs_imp_expr_eval brand_relation_brands σc (update_first equiv_dec σ v d') e').
-      Proof.
-        intros eqq Γc Γc_bt Γ Γ_bt  τ typ d d' inn ft.
-        revert e' eqq typ.
-        nnrs_imp_expr_cases (induction e) Case
-        ; simpl ; intros e' eqq typ
-        ; try discriminate.
-        - Case "NNRSimpVar"%string.
-          match_destr_in eqq.
-          invcs eqq; simpl.
-          rewrite e.
-          unfold var in *.
-          rewrite inn.
-          rewrite lookup_update_eq_in; eauto.
-          apply lookup_in_domain in inn; trivial.
-        - Case "NNRSimpConst"%string.
-          destruct d0; try discriminate.
+              lookup equiv_dec σ v = Some d ->
+              lift2P flattens_to d d' ->
+              lift2P
+                flattens_to
+                (nnrs_imp_expr_eval brand_relation_brands σc σ e)
+                (nnrs_imp_expr_eval brand_relation_brands σc (update_first equiv_dec σ v d') e').
+    Proof.
+      intros eqq Γc Γc_bt Γ Γ_bt  τ typ d d' inn ft.
+      revert e' eqq typ.
+      nnrs_imp_expr_cases (induction e) Case
+      ; simpl ; intros e' eqq typ
+      ; try discriminate.
+      - Case "NNRSimpVar"%string.
+        match_destr_in eqq.
+        invcs eqq; simpl.
+        rewrite e.
+        unfold var in *.
+        rewrite inn.
+        rewrite lookup_update_eq_in; eauto.
+        apply lookup_in_domain in inn; trivial.
+      - Case "NNRSimpConst"%string.
+        destruct d0; try discriminate.
+        destruct l; try discriminate.
+        + invcs eqq; simpl; reflexivity.
+        + destruct d0; try discriminate.
           destruct l; try discriminate.
-          + invcs eqq; simpl; reflexivity.
-          + destruct d0; try discriminate.
-             destruct l; try discriminate.
-             invcs eqq; simpl.
-             unfold oflatten; simpl.
-            rewrite app_nil_r; trivial.
-        - Case "NNRSimpBinop"%string.
-          destruct b; try discriminate.
-          apply some_lift2 in eqq.
-          destruct eqq as [?[? eqq1[eqq2 ?]]]; subst.
-          simpl.
-          invcs typ.
-          invcs H3.
-          apply Coll_right_inv in H; subst.
-          specialize (IHe1 _ eqq1 H5).
-          specialize (IHe2 _ eqq2 H6).
-          unfold lift2P in *; simpl.
-          repeat match_option_in IHe1
-          ; simpl in *
-          ; try contradiction.
-          repeat match_option_in IHe2
-          ; simpl in *
-          ; try contradiction.
+          invcs eqq; simpl.
+          unfold oflatten; simpl.
+          rewrite app_nil_r; trivial.
+      - Case "NNRSimpBinop"%string.
+        destruct b; try discriminate.
+        apply some_lift2 in eqq.
+        destruct eqq as [?[? eqq1[eqq2 ?]]]; subst.
+        simpl.
+        invcs typ.
+        invcs H3.
+        apply Coll_right_inv in H; subst.
+        specialize (IHe1 _ eqq1 H5).
+        specialize (IHe2 _ eqq2 H6).
+        unfold lift2P in *; simpl.
+        repeat match_option_in IHe1
+        ; simpl in *
+        ; try contradiction.
+        repeat match_option_in IHe2
+        ; simpl in *
+        ; try contradiction.
 
-          destruct d0; simpl in *; try contradiction
-          ; destruct d1; simpl in *; try contradiction
-          ; trivial.
-          destruct d2; simpl in *; try contradiction
-          ; destruct d3; simpl in *; try contradiction
-          ; trivial.
-          unfold bunion.
-          erewrite oflatten_app; eauto.
-        - Case "NNRSimpUnop"%string.
-          destruct u; simpl; try discriminate.
-          match_destr_in eqq.
-          invcs eqq.
-          invcs typ.
-          invcs H2.
-          apply Coll_right_inv in H.
-          rtype_equalizer; subst.
-          replace (nnrs_imp_expr_eval brand_relation_brands σc (update_first equiv_dec σ v d') e')
-            with (nnrs_imp_expr_eval brand_relation_brands σc σ e').
-          + 
-            case_eq (nnrs_imp_expr_eval brand_relation_brands σc σ e'); simpl; trivial.
-            intros ? eqq.
-            eapply nnrs_imp_expr_eval_preserves_types in eqq; eauto.
-            dtype_inverter.
-            rewrite oflatten_cons with (r':=nil); simpl; trivial.
-            rewrite app_nil_r; trivial.
-          + eapply nnrs_imp_expr_eval_same.
-            red; intros.
-            destruct (x == v).
-            * rewrite e in *; tauto.
-            * rewrite lookup_update_neq; eauto.
-      Qed.
+        destruct d0; simpl in *; try contradiction
+        ; destruct d1; simpl in *; try contradiction
+        ; trivial.
+        destruct d2; simpl in *; try contradiction
+        ; destruct d3; simpl in *; try contradiction
+        ; trivial.
+        unfold bunion.
+        erewrite oflatten_app; eauto.
+      - Case "NNRSimpUnop"%string.
+        destruct u; simpl; try discriminate.
+        match_destr_in eqq.
+        invcs eqq.
+        invcs typ.
+        invcs H2.
+        apply Coll_right_inv in H.
+        rtype_equalizer; subst.
+        replace (nnrs_imp_expr_eval brand_relation_brands σc (update_first equiv_dec σ v d') e')
+          with (nnrs_imp_expr_eval brand_relation_brands σc σ e').
+        + 
+          case_eq (nnrs_imp_expr_eval brand_relation_brands σc σ e'); simpl; trivial.
+          intros ? eqq.
+          eapply nnrs_imp_expr_eval_preserves_types in eqq; eauto.
+          dtype_inverter.
+          rewrite oflatten_cons with (r':=nil); simpl; trivial.
+          rewrite app_nil_r; trivial.
+        + eapply nnrs_imp_expr_eval_same.
+          red; intros.
+          destruct (x == v).
+          * rewrite e in *; tauto.
+          * rewrite lookup_update_neq; eauto.
+    Qed.
 
-          Ltac disect_tac H stac
-    := 
-      unfold var in *
-      ; cut_to H; unfold domain in *; [ | solve[stac]..]
-      ; unfold lift2P in H
-      ; (repeat match_option_in H; try contradiction).
+    Ltac disect_tac H stac
+      := 
+        unfold var in *
+        ; cut_to H; unfold domain in *; [ | solve[stac]..]
+        ; unfold lift2P in H
+        ; (repeat match_option_in H; try contradiction).
 
-  Ltac pcong
-    := solve[repeat (match goal with
-                     | [H: _ = _ |- _ ] => rewrite H in *; clear H
-                     end; try tauto)].
+    Ltac pcong
+      := solve[repeat (match goal with
+                       | [H: _ = _ |- _ ] => rewrite H in *; clear H
+                       end; try tauto)].
 
-  Ltac fuse_t stac
-    := repeat progress (
-                repeat rewrite in_app_iff in *
-                ; repeat
-                    match goal with
-                    | [H : ~ (_ \/ _ ) |- _ ] => apply not_or in H
-                    | [H : (_ \/ _ ) -> False |- _ ] => apply not_or in H
-                    | [H: _ /\ _ |- _ ] => destruct H
-                    | [ H : _ * _ |- _ ] => destruct H
-                    | [H: _::_ = _::_ |- _ ] => invcs H
-                    | [ H: domain (_ ++ _) = domain _ |- _ ] =>
-                      rewrite domain_app in H
-                      ; unfold domain in H
-                      ; symmetry in H; apply map_app_break in H
-                      ; destruct H as [? [?[?[??]]]]; subst; simpl in *
-                    | [ H: map (_ ++ _) = map _ |- _ ] =>
-                      rewrite map_app in H
-                      ; symmetry in H; apply map_app_break in H
-                      ; destruct H as [? [?[?[??]]]]; subst; simpl in *
-                    | [ H: _ :: _ = map _ ?x |- _ ] =>
-                      destruct x; try discriminate; simpl in H; invcs H
-                    | [ H: _ :: _ = domain ?x |- _ ] =>
-                      destruct x; try discriminate; simpl in H; invcs H
-                    | [H : ~ In _ (remove _ _ _) |- _ ] =>
-                      apply not_in_remove_impl_not_in in H; [| congruence]
-                    | [H : ?x ++ _ = ?y ++ _ |- _ ] =>
-                      let HH := fresh in
-                      assert (HH:domain y = domain x) by
-                          (unfold domain in *;
-                           try (intuition congruence)
-                           ; pcong)
-                      ; apply app_inv_head_domain in H;[clear HH|apply HH]
+    Ltac fuse_t stac
+      := repeat progress (
+                  repeat rewrite in_app_iff in *
+                  ; repeat
+                      match goal with
+                      | [H : ~ (_ \/ _ ) |- _ ] => apply not_or in H
+                      | [H : (_ \/ _ ) -> False |- _ ] => apply not_or in H
+                      | [H: _ /\ _ |- _ ] => destruct H
+                      | [ H : _ * _ |- _ ] => destruct H
+                      | [H: _::_ = _::_ |- _ ] => invcs H
+                      | [ H: domain (_ ++ _) = domain _ |- _ ] =>
+                        rewrite domain_app in H
+                        ; unfold domain in H
+                        ; symmetry in H; apply map_app_break in H
+                        ; destruct H as [? [?[?[??]]]]; subst; simpl in *
+                      | [ H: map (_ ++ _) = map _ |- _ ] =>
+                        rewrite map_app in H
+                        ; symmetry in H; apply map_app_break in H
+                        ; destruct H as [? [?[?[??]]]]; subst; simpl in *
+                      | [ H: _ :: _ = map _ ?x |- _ ] =>
+                        destruct x; try discriminate; simpl in H; invcs H
+                      | [ H: _ :: _ = domain ?x |- _ ] =>
+                        destruct x; try discriminate; simpl in H; invcs H
+                      | [H : ~ In _ (remove _ _ _) |- _ ] =>
+                        apply not_in_remove_impl_not_in in H; [| congruence]
+                      | [H : ?x ++ _ = ?y ++ _ |- _ ] =>
+                        let HH := fresh in
+                        assert (HH:domain y = domain x) by
+                            (unfold domain in *;
+                             try (intuition congruence)
+                             ; pcong)
+                        ; apply app_inv_head_domain in H;[clear HH|apply HH]
 
-                    | [ H: forall a b c, _ -> ?x1 :: ?dd :: ?x2 = _ ++ _ :: _ -> _ |- _] =>
-                      specialize (H (x1::nil) (snd dd) x2); simpl in H
-                      ; match dd with
-                        | (_,_) => idtac
-                        | _ => destruct dd
-                        end
-                      ; simpl in *
-                      ; cut_to H; [ | eauto 3 | reflexivity]
-                    end
-                ; simpl in *; trivial; intros; try subst; try contradiction; try solve [congruence | f_equal; congruence]).
+                      | [ H: forall a b c, _ -> ?x1 :: ?dd :: ?x2 = _ ++ _ :: _ -> _ |- _] =>
+                        specialize (H (x1::nil) (snd dd) x2); simpl in H
+                        ; match dd with
+                          | (_,_) => idtac
+                          | _ => destruct dd
+                          end
+                        ; simpl in *
+                        ; cut_to H; [ | eauto 3 | reflexivity]
+                      end
+                  ; simpl in *; trivial; intros; try subst; try contradiction; try solve [congruence | f_equal; congruence]).
 
     Ltac fuse_tt := fuse_t ltac:(try tauto; try congruence).
 
-      Lemma nnrs_imp_stmt_unflatten_eval s s' v σc σ d :
-        nnrs_imp_stmt_unflatten s v = Some s' ->
-        forall Γc,
-          bindings_type σc Γc ->
-          forall Γ,
-            pd_bindings_type σ Γ ->
-            forall τ,
-              lookup equiv_dec σ v = Some d ->
-              lookup equiv_dec Γ v = Some (Coll (Coll τ)) ->
-              [ Γc ; Γ  ⊢ s ] ->
-              forall d',
+    Lemma nnrs_imp_stmt_unflatten_eval s s' v σc σ d :
+      nnrs_imp_stmt_unflatten s v = Some s' ->
+      forall Γc,
+        bindings_type σc Γc ->
+        forall Γ,
+          pd_bindings_type σ Γ ->
+          forall τ,
+            lookup equiv_dec σ v = Some d ->
+            lookup equiv_dec Γ v = Some (Coll (Coll τ)) ->
+            [ Γc ; Γ  ⊢ s ] ->
+            forall d',
               lift2P flattens_to d d' ->
               lift2P
                 (fun σ₁' σ₂' =>
                    match lookup equiv_dec σ₁' v with
                    | Some dd => 
                      exists dd',
-                       σ₂' = update_first equiv_dec σ₁' v dd'
-                       /\ lift2P flattens_to dd dd'
+                     σ₂' = update_first equiv_dec σ₁' v dd'
+                     /\ lift2P flattens_to dd dd'
                    | None => False
                    end
                 )
                 (nnrs_imp_stmt_eval brand_relation_brands σc s σ)
                 (nnrs_imp_stmt_eval brand_relation_brands σc s' (update_first equiv_dec σ v d')).
-      Proof.
-        intros eqq Γc σc_bt.
-        revert s' σ d eqq.
-        nnrs_imp_stmt_cases (induction s) Case
-        ; simpl ; intros s' σ d eqq Γ σ_bt τ σinn Γinn typ d' ft.
-        - Case "NNRSimpSkip"%string.
-          invcs eqq; simpl; intros.
-          unfold var in *.
-          rewrite σinn.
-          eauto.
-        - Case "NNRSimpSeq"%string.
-          apply some_lift2 in eqq.
-          destruct eqq as [?[? eqq1 [eqq2 ?]] ]; subst; simpl.
+    Proof.
+      intros eqq Γc σc_bt.
+      revert s' σ d eqq.
+      nnrs_imp_stmt_cases (induction s) Case
+      ; simpl ; intros s' σ d eqq Γ σ_bt τ σinn Γinn typ d' ft.
+      - Case "NNRSimpSkip"%string.
+        invcs eqq; simpl; intros.
+        unfold var in *.
+        rewrite σinn.
+        eauto.
+      - Case "NNRSimpSeq"%string.
+        apply some_lift2 in eqq.
+        destruct eqq as [?[? eqq1 [eqq2 ?]] ]; subst; simpl.
+        invcs typ.
+        specialize (IHs1 _ _ _ eqq1 _ σ_bt _ σinn Γinn H2 _ ft).
+        unfold lift2P in *.
+        do 3 (match_option_in IHs1; simpl in *
+              ; try contradiction).
+        destruct IHs1 as [dd' [? ft']].
+        subst.
+        generalize (nnrs_imp_stmt_eval_preserves_types _ σc_bt σ_bt H2 _ eqq)
+        ; intros p_bt.
+        eapply IHs2; eauto.
+      - Case "NNRSimpAssign"%string.
+        destruct (equiv_dec v0 v); unfold equiv, complement in *.
+        + subst; simpl in *.
+          apply some_lift in eqq.
+          destruct eqq as [? eqq ?]; subst.
           invcs typ.
-          specialize (IHs1 _ _ _ eqq1 _ σ_bt _ σinn Γinn H2 _ ft).
-          unfold lift2P in *.
-          do 3 (match_option_in IHs1; simpl in *
-                ; try contradiction).
-          destruct IHs1 as [dd' [? ft']].
-          subst.
-          generalize (nnrs_imp_stmt_eval_preserves_types _ σc_bt σ_bt H2 _ eqq)
-          ; intros p_bt.
-          eapply IHs2; eauto.
-        - Case "NNRSimpAssign"%string.
-          destruct (equiv_dec v0 v); unfold equiv, complement in *.
-          + subst; simpl in *.
-            apply some_lift in eqq.
-            destruct eqq as [? eqq ?]; subst.
-            invcs typ.
-            unfold equiv_dec, string_eqdec in *.
-            rewrite Γinn in H3.
-            invcs H3.
-            generalize (nnrs_imp_expr_unflatten_write_eval _ _ _ _ _
-                                                           eqq _ σc_bt _ σ_bt _ H2 _ _ σinn ft)
-            ; intros ft'.
-            simpl.
-            unfold lift2P in ft'.
-            unfold equiv_dec, string_eqdec in *.
+          unfold equiv_dec, string_eqdec in *.
+          rewrite Γinn in H3.
+          invcs H3.
+          generalize (nnrs_imp_expr_unflatten_write_eval _ _ _ _ _
+                                                         eqq _ σc_bt _ σ_bt _ H2 _ _ σinn ft)
+          ; intros ft'.
+          simpl.
+          unfold lift2P in ft'.
+          unfold equiv_dec, string_eqdec in *.
 
-            repeat match_option_in ft'
+          repeat match_option_in ft'
           ; simpl in *
           ; try contradiction.
-            rewrite σinn.
-            simpl.
-            repeat rewrite lookup_update_eq_in.
-            * exists (Some d1).
-              repeat rewrite update_first_update_first_eq; simpl.
-              tauto.
-            * apply lookup_in_domain in σinn; trivial.
-            * apply lookup_in_domain in σinn; trivial.
-          + apply some_lift in eqq.
-             destruct eqq as [? eqq ?]; subst.
-             invcs typ.
-            rewrite (nnrs_imp_expr_unflatten_read_eval _ _ _ brand_relation_brands σc _ _ _
-                                                       eqq σinn ft).
-            simpl.
-            unfold equiv_dec, string_eqdec, var in *.
-            match_option; simpl; trivial.
-            rewrite lookup_update_neq by eauto.
-            match_option; simpl; trivial.
-            rewrite lookup_update_neq by eauto.
-            rewrite σinn.
-            exists d'.
-            split; trivial.
-            rewrite update_first_update_first_neq_swap; eauto.
-        - Case "NNRSimpLet"%string.
-          apply some_lift2 in eqq.
-          destruct eqq as [?[? eqq1 [eqq2 ?]] ]; subst; simpl.
+          rewrite σinn.
+          simpl.
+          repeat rewrite lookup_update_eq_in.
+          * exists (Some d1).
+            repeat rewrite update_first_update_first_eq; simpl.
+            tauto.
+          * apply lookup_in_domain in σinn; trivial.
+          * apply lookup_in_domain in σinn; trivial.
+        + apply some_lift in eqq.
+          destruct eqq as [? eqq ?]; subst.
           invcs typ.
-          + simpl in eqq1.
-            apply some_lift in eqq1.
-            destruct eqq1 as [? eqq1 ?]; subst.
-            rewrite <- (nnrs_imp_expr_unflatten_read_eval _ _ _ brand_relation_brands σc _ _ _
-                                                            eqq1 σinn ft).
-            case_eq (nnrs_imp_expr_eval brand_relation_brands σc σ e₁); simpl; trivial
-            ; intros ? eveqq.
-            match_destr_in eqq2; unfold equiv, complement in *.
-            * subst.
-              invcs eqq2.
-              destruct (in_update_break_first _ σinn d')
-                as [?[? [? [eqq2 nin]]]]
-              ; subst.
-              rewrite eqq2.
-              generalize (nnrs_imp_stmt_eval_unused brand_relation_brands σc ((v, Some d0)::x) x2 x0 v d)
-              ; simpl ; intros HH1.
-              cut_to HH1; [| tauto].
-              generalize (nnrs_imp_stmt_eval_unused brand_relation_brands σc ((v, Some d0)::x) x2 x0 v d')
-              ; simpl ; intros HH2.
-              cut_to HH2; [| tauto].
-              unfold lift2P, var in *.
-              repeat match_option_in HH1
-              ; rewrite eqq0 in HH2
-              ; try contradiction
-              ; repeat match_option_in HH2
-              ; try contradiction.
-              apply nnrs_imp_stmt_eval_domain_stack in eqq.
-              apply nnrs_imp_stmt_eval_domain_stack in eqq3.
-              fuse_tt.
-              rewrite lookup_app.
-              rewrite lookup_nin_none; [|  unfold domain in *; congruence].
-              simpl.
-              destruct (equiv_dec s s); [| congruence].
-              exists o0.
-              rewrite update_app_nin; [|  unfold domain in *; congruence].
-              simpl.
-              destruct (equiv_dec s s); [| congruence].
-              specialize (HH1 ((s,o1)::x5) o2 x6); simpl in HH1.
-              cut_to HH1; [| unfold domain in *; congruence | trivial].
-              specialize (HH2 ((s,o)::x3) o0 x4); simpl in HH2.
-              cut_to HH2; [| unfold domain in *; congruence | trivial].
-              destruct HH1; subst.
-              fuse_tt.
-              split; trivial.
-            * assert (σ_bt_cons : pd_bindings_type ((v0, Some d0) :: σ) ((v0, τ0) :: Γ)).
-              {
-                econstructor; simpl; trivial.
-                split; trivial; intros.
-                invcs H.
-                eapply nnrs_imp_expr_eval_preserves_types  in eveqq; eauto.
-              } 
-              specialize (IHs _ ((v0, Some d0)::σ) d eqq2 ((v0, τ0) :: Γ) σ_bt_cons τ).
-              cut_to IHs; simpl; trivial; try solve [match_destr; congruence].
-              specialize (IHs _ ft).
-              simpl in IHs.
-              unfold var in *.
-              destruct (equiv_dec v v0); try congruence.
-              unfold lift2P in *.
-              do 2 match_option_in IHs
-              ; try contradiction.
-              generalize (nnrs_imp_stmt_eval_domain_stack eqq)
-              ; generalize (nnrs_imp_stmt_eval_domain_stack eqq0)
-              ; intros.
-              fuse_tt.
-              destruct (equiv_dec v s0); [congruence| ].
-              match_option_in IHs.
-              destruct IHs as [dd' [HH1 HH2]].
-              invcs HH1.
-              exists dd'; split; trivial.
-          + simpl in eqq1; invcs eqq1.
-            match_destr_in eqq2; unfold equiv, complement in *.
-            * subst.
-              invcs eqq2.
-              destruct (in_update_break_first _ σinn d')
-                as [?[? [? [eqq2 nin]]]]
-              ; subst.
-              rewrite eqq2.
-              generalize (nnrs_imp_stmt_eval_unused brand_relation_brands σc ((v, None)::x) x1 x0 v d)
-              ; simpl ; intros HH1.
-              cut_to HH1; [| tauto].
-              generalize (nnrs_imp_stmt_eval_unused brand_relation_brands σc ((v, None)::x) x1 x0 v d')
-              ; simpl ; intros HH2.
-              cut_to HH2; [| tauto].
-              unfold lift2P, var in *.
-              repeat match_option_in HH1
-              ; rewrite eqq0 in HH2
-              ; try contradiction
-              ; repeat match_option_in HH2
-              ; try contradiction.
-              apply nnrs_imp_stmt_eval_domain_stack in eqq.
-              apply nnrs_imp_stmt_eval_domain_stack in eqq1.
-              fuse_tt.
-              rewrite lookup_app.
-              rewrite lookup_nin_none; [|  unfold domain in *; congruence].
-              simpl.
-              destruct (equiv_dec s s); [| congruence].
-              exists o0.
-              rewrite update_app_nin; [|  unfold domain in *; congruence].
-              simpl.
-              destruct (equiv_dec s s); [| congruence].
-              specialize (HH1 ((s,o1)::x4) o2 x5); simpl in HH1.
-              cut_to HH1; [| unfold domain in *; congruence | trivial].
-              specialize (HH2 ((s,o)::x2) o0 x3); simpl in HH2.
-              cut_to HH2; [| unfold domain in *; congruence | trivial].
-              destruct HH1; subst.
-              fuse_tt.
-              split; trivial.
-            * assert (σ_bt_cons : pd_bindings_type ((v0, None) :: σ) ((v0, τ0) :: Γ)).
-              {
-                econstructor; simpl; trivial.
-                split; trivial; intros.
-                invcs H.
-              } 
-              specialize (IHs _ ((v0, None)::σ) d eqq2 ((v0, τ0) :: Γ) σ_bt_cons τ).
-              cut_to IHs; simpl; trivial; try solve [match_destr; congruence].
-              specialize (IHs _ ft).
-              simpl in IHs.
-              unfold var in *.
-              destruct (equiv_dec v v0); try congruence.
-              unfold lift2P in *.
-              do 2 match_option_in IHs
-              ; try contradiction.
-              generalize (nnrs_imp_stmt_eval_domain_stack eqq)
-              ; generalize (nnrs_imp_stmt_eval_domain_stack eqq0)
-              ; intros.
-              fuse_tt.
-              destruct (equiv_dec v s0); [congruence| ].
-              match_option_in IHs.
-              destruct IHs as [dd' [HH1 HH2]].
-              invcs HH1.
-              exists dd'; split; trivial.
-        - Case "NNRSimpFor"%string.
-          apply some_lift2 in eqq.
-          destruct eqq as [?[? eqq1 [eqq2 ?]] ]; subst; simpl.
-          invcs typ.
+          rewrite (nnrs_imp_expr_unflatten_read_eval _ _ _ brand_relation_brands σc _ _ _
+                                                     eqq σinn ft).
+          simpl.
+          unfold equiv_dec, string_eqdec, var in *.
+          match_option; simpl; trivial.
+          rewrite lookup_update_neq by eauto.
+          match_option; simpl; trivial.
+          rewrite lookup_update_neq by eauto.
+          rewrite σinn.
+          exists d'.
+          split; trivial.
+          rewrite update_first_update_first_neq_swap; eauto.
+      - Case "NNRSimpLet"%string.
+        apply some_lift2 in eqq.
+        destruct eqq as [?[? eqq1 [eqq2 ?]] ]; subst; simpl.
+        invcs typ.
+        + simpl in eqq1.
+          apply some_lift in eqq1.
+          destruct eqq1 as [? eqq1 ?]; subst.
           rewrite <- (nnrs_imp_expr_unflatten_read_eval _ _ _ brand_relation_brands σc _ _ _
                                                         eqq1 σinn ft).
-          case_eq (nnrs_imp_expr_eval brand_relation_brands σc σ n); simpl; trivial
+          case_eq (nnrs_imp_expr_eval brand_relation_brands σc σ e₁); simpl; trivial
           ; intros ? eveqq.
-          eapply nnrs_imp_expr_eval_preserves_types  in eveqq; eauto.
-          dtype_inverter.
-          invcs eveqq; rtype_equalizer; subst.
-          clear x n eqq1 H2.
-          revert σ Γ d d' σinn σ_bt H4 Γinn ft.
-          induction d0; intros σ Γ d d' σinn σ_bt typ Γinn ft; simpl; unfold var in *.
-          + rewrite σinn; eauto.
-          + invcs H1.
-            specialize (IHd0 H3); clear H3.
-            match_destr_in eqq2; unfold equiv, complement in *.
-            * subst.
-              invcs eqq2.
-              destruct (in_update_break_first _ σinn d')
-                as [?[? [? [eqq2 nin]]]]
-              ; subst.
-              rewrite eqq2.
-              clear eqq2.
-              generalize (nnrs_imp_stmt_eval_unused brand_relation_brands σc ((v, Some a)::x) x1 x0 v d)
-              ; simpl ; intros HH1.
-              cut_to HH1; [| tauto].
-              generalize (nnrs_imp_stmt_eval_unused brand_relation_brands σc ((v, Some a)::x) x1 x0 v d')
-              ; simpl ; intros HH2.
-              cut_to HH2; [| tauto].
-              unfold lift2P, var in *.
-              repeat match_option_in HH1
-              ; rewrite eqq0 in HH2
-              ; try contradiction
-              ; repeat match_option_in HH2
-              ; try contradiction.
-              generalize (nnrs_imp_stmt_eval_domain_stack eqq).
-              generalize (nnrs_imp_stmt_eval_domain_stack eqq1).
-              fuse_tt.
-              specialize (HH1 ((s,o)::x2) o0 x3); simpl in HH1.
-              cut_to HH1; [| unfold domain in *; congruence | trivial].
-              specialize (HH2 ((s,o1)::x4) o2 x5); simpl in HH2.
-              cut_to HH2; [| unfold domain in *; congruence | trivial].
-              destruct HH1; subst.
-              fuse_tt.
-              { eapply nnrs_imp_stmt_eval_preserves_types  in eqq; eauto.
-                - specialize (IHd0 (x4 ++ (s, o0) :: x5) Γ o0 o2).
-                  { cut_to IHd0; trivial.
-                - unfold lift2P in *.
-                  rewrite update_app_nin in IHd0; [ | unfold domain in *; congruence].
-                  simpl in IHd0.
-                  destruct (equiv_dec s s); [| congruence].
-                  trivial.
-                - rewrite lookup_app.
-                  rewrite lookup_nin_none; simpl.
-                  + destruct (equiv_dec s s); [| congruence]; trivial.
-                  + unfold domain in *; congruence.
-                - invcs eqq; auto.
-                  } 
-                - econstructor; simpl; trivial; split; trivial; intros ? eqqq; invcs eqqq; trivial.
-              }
-            * assert (σ_bt_cons : pd_bindings_type ((v0, Some a) :: σ) ((v0, τ0) :: Γ)).
-              {
-                econstructor; simpl; trivial.
-                split; trivial; intros.
-                invcs H; trivial.
-              } 
-              specialize (IHs _ ((v0, Some a)::σ) d eqq2 ((v0, τ0) :: Γ) σ_bt_cons τ).
-              cut_to IHs; simpl; trivial; try solve [match_destr; congruence].
-              specialize (IHs _ ft).
-              simpl in IHs.
-              unfold var in *.
-              destruct (equiv_dec v v0); try congruence.
-              unfold lift2P in *.
-              do 2 match_option_in IHs
-              ; try contradiction.
-              generalize (nnrs_imp_stmt_eval_domain_stack eqq)
-              ; generalize (nnrs_imp_stmt_eval_domain_stack eqq0)
-              ; intros.
-              fuse_tt.
-              destruct (equiv_dec v s0); [congruence| ].
-              match_option_in IHs; try contradiction.
-              destruct IHs as [dd' [HH1 HH2]].
-              invcs HH1.
-              clear H3.
-              generalize (nnrs_imp_stmt_eval_preserves_types _ σc_bt σ_bt_cons typ _ eqq)
-              ; intros p_bt.
-              invcs p_bt.
-              specialize (IHd0 p1 Γ o1 dd').
-              cut_to IHd0; trivial.
-        - Case "NNRSimpIf"%string.
-          unfold lift3 in eqq.
-          repeat match_option_in eqq.
-          invcs eqq; simpl in *.
-          invcs typ.
-          rewrite <- (nnrs_imp_expr_unflatten_read_eval _ _ _ brand_relation_brands σc _ _ _
-                                                     eqq0 σinn ft).
-          match_option; simpl; trivial.
-          destruct d0; simpl; trivial.
-          destruct b; eauto.
-        - Case "NNRSimpEither"%string.
-          unfold lift3 in eqq.
-          repeat match_option_in eqq.
-          invcs eqq; simpl in *.
-          invcs typ.
-          rewrite <- (nnrs_imp_expr_unflatten_read_eval _ _ _ brand_relation_brands σc _ _ _
-                                                     eqq0 σinn ft).
-          match_option; simpl; trivial.
-          eapply nnrs_imp_expr_eval_preserves_types  in eqq; eauto.
-          destruct d0; simpl; trivial
-          ; invcs eqq; rtype_equalizer; subst.
-          + match_destr_in eqq1; unfold equiv, complement in *.
-            * subst.
-              invcs eqq1.
-              destruct (in_update_break_first _ σinn d')
-                as [?[? [? [eqq1 nin]]]]
-              ; subst.
-              rewrite eqq1.
-              generalize (nnrs_imp_stmt_eval_unused brand_relation_brands σc ((v, Some d0)::x) x0 n1 v d)
-              ; simpl ; intros HH1.
-              cut_to HH1; [| tauto].
-              generalize (nnrs_imp_stmt_eval_unused brand_relation_brands σc ((v, Some d0)::x) x0 n1 v d')
-              ; simpl ; intros HH2.
-              cut_to HH2; [| tauto].
-              unfold lift2P, var in *.
-              repeat match_option_in HH1
-              ; rewrite eqq3 in HH2
-              ; try contradiction
-              ; repeat match_option_in HH2
-              ; try contradiction.
-              apply nnrs_imp_stmt_eval_domain_stack in eqq.
-              apply nnrs_imp_stmt_eval_domain_stack in eqq4.
-              fuse_tt.
-              rewrite lookup_app.
-              rewrite lookup_nin_none; [|  unfold domain in *; congruence].
-              simpl.
-              destruct (equiv_dec s s); [| congruence].
-              exists o0.
-              rewrite update_app_nin; [|  unfold domain in *; congruence].
-              simpl.
-              destruct (equiv_dec s s); [| congruence].
-              specialize (HH1 ((s,o1)::x3) o2 x4); simpl in HH1.
-              cut_to HH1; [| unfold domain in *; congruence | trivial].
-              specialize (HH2 ((s,o)::x1) o0 x2); simpl in HH2.
-              cut_to HH2; [| unfold domain in *; congruence | trivial].
-              destruct HH1; subst.
-              fuse_tt.
-              split; trivial.
-            * assert (σ_bt_cons : pd_bindings_type ((v0, Some d0) :: σ) ((v0, τl) :: Γ)).
-              {
-                econstructor; simpl; trivial.
-                split; trivial; intros.
-                invcs H; trivial.
-              } 
-              specialize (IHs1 _ ((v0, Some d0)::σ) d eqq1 ((v0, τl) :: Γ) σ_bt_cons τ).
-              cut_to IHs1; simpl; trivial; try solve [match_destr; congruence].
-              specialize (IHs1 _ ft).
-              simpl in IHs1.
-              unfold var in *.
-              destruct (equiv_dec v v0); try congruence.
-              unfold lift2P in *.
-              do 2 match_option_in IHs1
-              ; try contradiction.
-              generalize (nnrs_imp_stmt_eval_domain_stack eqq)
-              ; generalize (nnrs_imp_stmt_eval_domain_stack eqq3)
-              ; intros.
-              fuse_tt.
-              destruct (equiv_dec v s); [congruence| ].
-              match_option_in IHs1.
-              destruct IHs1 as [dd' [HH1 HH2]].
-              invcs HH1.
-              exists dd'; split; trivial. 
-          + match_destr_in eqq2; unfold equiv, complement in *.
-            * subst.
-              invcs eqq2.
-              destruct (in_update_break_first _ σinn d')
-                as [?[? [? [eqq2 nin]]]]
-              ; subst.
-              rewrite eqq2.
-              generalize (nnrs_imp_stmt_eval_unused brand_relation_brands σc ((v, Some d0)::x) x0 n2 v d)
-              ; simpl ; intros HH1.
-              cut_to HH1; [| tauto].
-              generalize (nnrs_imp_stmt_eval_unused brand_relation_brands σc ((v, Some d0)::x) x0 n2 v d')
-              ; simpl ; intros HH2.
-              cut_to HH2; [| tauto].
-              unfold lift2P, var in *.
-              repeat match_option_in HH1
-              ; rewrite eqq3 in HH2
-              ; try contradiction
-              ; repeat match_option_in HH2
-              ; try contradiction.
-              apply nnrs_imp_stmt_eval_domain_stack in eqq.
-              apply nnrs_imp_stmt_eval_domain_stack in eqq4.
-              fuse_tt.
-              rewrite lookup_app.
-              rewrite lookup_nin_none; [|  unfold domain in *; congruence].
-              simpl.
-              destruct (equiv_dec s s); [| congruence].
-              exists o0.
-              rewrite update_app_nin; [|  unfold domain in *; congruence].
-              simpl.
-              destruct (equiv_dec s s); [| congruence].
-              specialize (HH1 ((s,o1)::x3) o2 x4); simpl in HH1.
-              cut_to HH1; [| unfold domain in *; congruence | trivial].
-              specialize (HH2 ((s,o)::x1) o0 x2); simpl in HH2.
-              cut_to HH2; [| unfold domain in *; congruence | trivial].
-              destruct HH1; subst.
-              fuse_tt.
-              split; trivial.
-            * assert (σ_bt_cons : pd_bindings_type ((v1, Some d0) :: σ) ((v1, τr) :: Γ)).
-              {
-                econstructor; simpl; trivial.
-                split; trivial; intros.
-                invcs H; trivial.
-              } 
-              specialize (IHs2 _ ((v1, Some d0)::σ) d eqq2 ((v1, τr) :: Γ) σ_bt_cons τ).
-              cut_to IHs2; simpl; trivial; try solve [match_destr; congruence].
-              specialize (IHs2 _ ft).
-              simpl in IHs2.
-              unfold var in *.
-              destruct (equiv_dec v v1); try congruence.
-              unfold lift2P in *.
-              do 2 match_option_in IHs2
-              ; try contradiction.
-              generalize (nnrs_imp_stmt_eval_domain_stack eqq)
-              ; generalize (nnrs_imp_stmt_eval_domain_stack eqq3)
-              ; intros.
-              fuse_tt.
-              destruct (equiv_dec v s); [congruence| ].
-              match_option_in IHs2.
-              destruct IHs2 as [dd' [HH1 HH2]].
-              invcs HH1.
-              exists dd'; split; trivial. 
-      Qed.
+          match_destr_in eqq2; unfold equiv, complement in *.
+          * subst.
+            invcs eqq2.
+            destruct (in_update_break_first _ σinn d')
+              as [?[? [? [eqq2 nin]]]]
+            ; subst.
+            rewrite eqq2.
+            generalize (nnrs_imp_stmt_eval_unused brand_relation_brands σc ((v, Some d0)::x) x2 x0 v d)
+            ; simpl ; intros HH1.
+            cut_to HH1; [| tauto].
+            generalize (nnrs_imp_stmt_eval_unused brand_relation_brands σc ((v, Some d0)::x) x2 x0 v d')
+            ; simpl ; intros HH2.
+            cut_to HH2; [| tauto].
+            unfold lift2P, var in *.
+            repeat match_option_in HH1
+            ; rewrite eqq0 in HH2
+            ; try contradiction
+            ; repeat match_option_in HH2
+            ; try contradiction.
+            apply nnrs_imp_stmt_eval_domain_stack in eqq.
+            apply nnrs_imp_stmt_eval_domain_stack in eqq3.
+            fuse_tt.
+            rewrite lookup_app.
+            rewrite lookup_nin_none; [|  unfold domain in *; congruence].
+            simpl.
+            destruct (equiv_dec s s); [| congruence].
+            exists o0.
+            rewrite update_app_nin; [|  unfold domain in *; congruence].
+            simpl.
+            destruct (equiv_dec s s); [| congruence].
+            specialize (HH1 ((s,o1)::x5) o2 x6); simpl in HH1.
+            cut_to HH1; [| unfold domain in *; congruence | trivial].
+            specialize (HH2 ((s,o)::x3) o0 x4); simpl in HH2.
+            cut_to HH2; [| unfold domain in *; congruence | trivial].
+            destruct HH1; subst.
+            fuse_tt.
+            split; trivial.
+          * assert (σ_bt_cons : pd_bindings_type ((v0, Some d0) :: σ) ((v0, τ0) :: Γ)).
+            {
+              econstructor; simpl; trivial.
+              split; trivial; intros.
+              invcs H.
+              eapply nnrs_imp_expr_eval_preserves_types  in eveqq; eauto.
+            } 
+            specialize (IHs _ ((v0, Some d0)::σ) d eqq2 ((v0, τ0) :: Γ) σ_bt_cons τ).
+            cut_to IHs; simpl; trivial; try solve [match_destr; congruence].
+            specialize (IHs _ ft).
+            simpl in IHs.
+            unfold var in *.
+            destruct (equiv_dec v v0); try congruence.
+            unfold lift2P in *.
+            do 2 match_option_in IHs
+            ; try contradiction.
+            generalize (nnrs_imp_stmt_eval_domain_stack eqq)
+            ; generalize (nnrs_imp_stmt_eval_domain_stack eqq0)
+            ; intros.
+            fuse_tt.
+            destruct (equiv_dec v s0); [congruence| ].
+            match_option_in IHs.
+            destruct IHs as [dd' [HH1 HH2]].
+            invcs HH1.
+            exists dd'; split; trivial.
+        + simpl in eqq1; invcs eqq1.
+          match_destr_in eqq2; unfold equiv, complement in *.
+          * subst.
+            invcs eqq2.
+            destruct (in_update_break_first _ σinn d')
+              as [?[? [? [eqq2 nin]]]]
+            ; subst.
+            rewrite eqq2.
+            generalize (nnrs_imp_stmt_eval_unused brand_relation_brands σc ((v, None)::x) x1 x0 v d)
+            ; simpl ; intros HH1.
+            cut_to HH1; [| tauto].
+            generalize (nnrs_imp_stmt_eval_unused brand_relation_brands σc ((v, None)::x) x1 x0 v d')
+            ; simpl ; intros HH2.
+            cut_to HH2; [| tauto].
+            unfold lift2P, var in *.
+            repeat match_option_in HH1
+            ; rewrite eqq0 in HH2
+            ; try contradiction
+            ; repeat match_option_in HH2
+            ; try contradiction.
+            apply nnrs_imp_stmt_eval_domain_stack in eqq.
+            apply nnrs_imp_stmt_eval_domain_stack in eqq1.
+            fuse_tt.
+            rewrite lookup_app.
+            rewrite lookup_nin_none; [|  unfold domain in *; congruence].
+            simpl.
+            destruct (equiv_dec s s); [| congruence].
+            exists o0.
+            rewrite update_app_nin; [|  unfold domain in *; congruence].
+            simpl.
+            destruct (equiv_dec s s); [| congruence].
+            specialize (HH1 ((s,o1)::x4) o2 x5); simpl in HH1.
+            cut_to HH1; [| unfold domain in *; congruence | trivial].
+            specialize (HH2 ((s,o)::x2) o0 x3); simpl in HH2.
+            cut_to HH2; [| unfold domain in *; congruence | trivial].
+            destruct HH1; subst.
+            fuse_tt.
+            split; trivial.
+          * assert (σ_bt_cons : pd_bindings_type ((v0, None) :: σ) ((v0, τ0) :: Γ)).
+            {
+              econstructor; simpl; trivial.
+              split; trivial; intros.
+              invcs H.
+            } 
+            specialize (IHs _ ((v0, None)::σ) d eqq2 ((v0, τ0) :: Γ) σ_bt_cons τ).
+            cut_to IHs; simpl; trivial; try solve [match_destr; congruence].
+            specialize (IHs _ ft).
+            simpl in IHs.
+            unfold var in *.
+            destruct (equiv_dec v v0); try congruence.
+            unfold lift2P in *.
+            do 2 match_option_in IHs
+            ; try contradiction.
+            generalize (nnrs_imp_stmt_eval_domain_stack eqq)
+            ; generalize (nnrs_imp_stmt_eval_domain_stack eqq0)
+            ; intros.
+            fuse_tt.
+            destruct (equiv_dec v s0); [congruence| ].
+            match_option_in IHs.
+            destruct IHs as [dd' [HH1 HH2]].
+            invcs HH1.
+            exists dd'; split; trivial.
+      - Case "NNRSimpFor"%string.
+        apply some_lift2 in eqq.
+        destruct eqq as [?[? eqq1 [eqq2 ?]] ]; subst; simpl.
+        invcs typ.
+        rewrite <- (nnrs_imp_expr_unflatten_read_eval _ _ _ brand_relation_brands σc _ _ _
+                                                      eqq1 σinn ft).
+        case_eq (nnrs_imp_expr_eval brand_relation_brands σc σ n); simpl; trivial
+        ; intros ? eveqq.
+        eapply nnrs_imp_expr_eval_preserves_types  in eveqq; eauto.
+        dtype_inverter.
+        invcs eveqq; rtype_equalizer; subst.
+        clear x n eqq1 H2.
+        revert σ Γ d d' σinn σ_bt H4 Γinn ft.
+        induction d0; intros σ Γ d d' σinn σ_bt typ Γinn ft; simpl; unfold var in *.
+        + rewrite σinn; eauto.
+        + invcs H1.
+          specialize (IHd0 H3); clear H3.
+          match_destr_in eqq2; unfold equiv, complement in *.
+          * subst.
+            invcs eqq2.
+            destruct (in_update_break_first _ σinn d')
+              as [?[? [? [eqq2 nin]]]]
+            ; subst.
+            rewrite eqq2.
+            clear eqq2.
+            generalize (nnrs_imp_stmt_eval_unused brand_relation_brands σc ((v, Some a)::x) x1 x0 v d)
+            ; simpl ; intros HH1.
+            cut_to HH1; [| tauto].
+            generalize (nnrs_imp_stmt_eval_unused brand_relation_brands σc ((v, Some a)::x) x1 x0 v d')
+            ; simpl ; intros HH2.
+            cut_to HH2; [| tauto].
+            unfold lift2P, var in *.
+            repeat match_option_in HH1
+            ; rewrite eqq0 in HH2
+            ; try contradiction
+            ; repeat match_option_in HH2
+            ; try contradiction.
+            generalize (nnrs_imp_stmt_eval_domain_stack eqq).
+            generalize (nnrs_imp_stmt_eval_domain_stack eqq1).
+            fuse_tt.
+            specialize (HH1 ((s,o)::x2) o0 x3); simpl in HH1.
+            cut_to HH1; [| unfold domain in *; congruence | trivial].
+            specialize (HH2 ((s,o1)::x4) o2 x5); simpl in HH2.
+            cut_to HH2; [| unfold domain in *; congruence | trivial].
+            destruct HH1; subst.
+            fuse_tt.
+            { eapply nnrs_imp_stmt_eval_preserves_types  in eqq; eauto.
+              - specialize (IHd0 (x4 ++ (s, o0) :: x5) Γ o0 o2).
+                { cut_to IHd0; trivial.
+                  - unfold lift2P in *.
+                    rewrite update_app_nin in IHd0; [ | unfold domain in *; congruence].
+                    simpl in IHd0.
+                    destruct (equiv_dec s s); [| congruence].
+                    trivial.
+                  - rewrite lookup_app.
+                    rewrite lookup_nin_none; simpl.
+                    + destruct (equiv_dec s s); [| congruence]; trivial.
+                    + unfold domain in *; congruence.
+                  - invcs eqq; auto.
+                } 
+              - econstructor; simpl; trivial; split; trivial; intros ? eqqq; invcs eqqq; trivial.
+            }
+          * assert (σ_bt_cons : pd_bindings_type ((v0, Some a) :: σ) ((v0, τ0) :: Γ)).
+            {
+              econstructor; simpl; trivial.
+              split; trivial; intros.
+              invcs H; trivial.
+            } 
+            specialize (IHs _ ((v0, Some a)::σ) d eqq2 ((v0, τ0) :: Γ) σ_bt_cons τ).
+            cut_to IHs; simpl; trivial; try solve [match_destr; congruence].
+            specialize (IHs _ ft).
+            simpl in IHs.
+            unfold var in *.
+            destruct (equiv_dec v v0); try congruence.
+            unfold lift2P in *.
+            do 2 match_option_in IHs
+            ; try contradiction.
+            generalize (nnrs_imp_stmt_eval_domain_stack eqq)
+            ; generalize (nnrs_imp_stmt_eval_domain_stack eqq0)
+            ; intros.
+            fuse_tt.
+            destruct (equiv_dec v s0); [congruence| ].
+            match_option_in IHs; try contradiction.
+            destruct IHs as [dd' [HH1 HH2]].
+            invcs HH1.
+            clear H3.
+            generalize (nnrs_imp_stmt_eval_preserves_types _ σc_bt σ_bt_cons typ _ eqq)
+            ; intros p_bt.
+            invcs p_bt.
+            specialize (IHd0 p1 Γ o1 dd').
+            cut_to IHd0; trivial.
+      - Case "NNRSimpIf"%string.
+        unfold lift3 in eqq.
+        repeat match_option_in eqq.
+        invcs eqq; simpl in *.
+        invcs typ.
+        rewrite <- (nnrs_imp_expr_unflatten_read_eval _ _ _ brand_relation_brands σc _ _ _
+                                                      eqq0 σinn ft).
+        match_option; simpl; trivial.
+        destruct d0; simpl; trivial.
+        destruct b; eauto.
+      - Case "NNRSimpEither"%string.
+        unfold lift3 in eqq.
+        repeat match_option_in eqq.
+        invcs eqq; simpl in *.
+        invcs typ.
+        rewrite <- (nnrs_imp_expr_unflatten_read_eval _ _ _ brand_relation_brands σc _ _ _
+                                                      eqq0 σinn ft).
+        match_option; simpl; trivial.
+        eapply nnrs_imp_expr_eval_preserves_types  in eqq; eauto.
+        destruct d0; simpl; trivial
+        ; invcs eqq; rtype_equalizer; subst.
+        + match_destr_in eqq1; unfold equiv, complement in *.
+          * subst.
+            invcs eqq1.
+            destruct (in_update_break_first _ σinn d')
+              as [?[? [? [eqq1 nin]]]]
+            ; subst.
+            rewrite eqq1.
+            generalize (nnrs_imp_stmt_eval_unused brand_relation_brands σc ((v, Some d0)::x) x0 n1 v d)
+            ; simpl ; intros HH1.
+            cut_to HH1; [| tauto].
+            generalize (nnrs_imp_stmt_eval_unused brand_relation_brands σc ((v, Some d0)::x) x0 n1 v d')
+            ; simpl ; intros HH2.
+            cut_to HH2; [| tauto].
+            unfold lift2P, var in *.
+            repeat match_option_in HH1
+            ; rewrite eqq3 in HH2
+            ; try contradiction
+            ; repeat match_option_in HH2
+            ; try contradiction.
+            apply nnrs_imp_stmt_eval_domain_stack in eqq.
+            apply nnrs_imp_stmt_eval_domain_stack in eqq4.
+            fuse_tt.
+            rewrite lookup_app.
+            rewrite lookup_nin_none; [|  unfold domain in *; congruence].
+            simpl.
+            destruct (equiv_dec s s); [| congruence].
+            exists o0.
+            rewrite update_app_nin; [|  unfold domain in *; congruence].
+            simpl.
+            destruct (equiv_dec s s); [| congruence].
+            specialize (HH1 ((s,o1)::x3) o2 x4); simpl in HH1.
+            cut_to HH1; [| unfold domain in *; congruence | trivial].
+            specialize (HH2 ((s,o)::x1) o0 x2); simpl in HH2.
+            cut_to HH2; [| unfold domain in *; congruence | trivial].
+            destruct HH1; subst.
+            fuse_tt.
+            split; trivial.
+          * assert (σ_bt_cons : pd_bindings_type ((v0, Some d0) :: σ) ((v0, τl) :: Γ)).
+            {
+              econstructor; simpl; trivial.
+              split; trivial; intros.
+              invcs H; trivial.
+            } 
+            specialize (IHs1 _ ((v0, Some d0)::σ) d eqq1 ((v0, τl) :: Γ) σ_bt_cons τ).
+            cut_to IHs1; simpl; trivial; try solve [match_destr; congruence].
+            specialize (IHs1 _ ft).
+            simpl in IHs1.
+            unfold var in *.
+            destruct (equiv_dec v v0); try congruence.
+            unfold lift2P in *.
+            do 2 match_option_in IHs1
+            ; try contradiction.
+            generalize (nnrs_imp_stmt_eval_domain_stack eqq)
+            ; generalize (nnrs_imp_stmt_eval_domain_stack eqq3)
+            ; intros.
+            fuse_tt.
+            destruct (equiv_dec v s); [congruence| ].
+            match_option_in IHs1.
+            destruct IHs1 as [dd' [HH1 HH2]].
+            invcs HH1.
+            exists dd'; split; trivial. 
+        + match_destr_in eqq2; unfold equiv, complement in *.
+          * subst.
+            invcs eqq2.
+            destruct (in_update_break_first _ σinn d')
+              as [?[? [? [eqq2 nin]]]]
+            ; subst.
+            rewrite eqq2.
+            generalize (nnrs_imp_stmt_eval_unused brand_relation_brands σc ((v, Some d0)::x) x0 n2 v d)
+            ; simpl ; intros HH1.
+            cut_to HH1; [| tauto].
+            generalize (nnrs_imp_stmt_eval_unused brand_relation_brands σc ((v, Some d0)::x) x0 n2 v d')
+            ; simpl ; intros HH2.
+            cut_to HH2; [| tauto].
+            unfold lift2P, var in *.
+            repeat match_option_in HH1
+            ; rewrite eqq3 in HH2
+            ; try contradiction
+            ; repeat match_option_in HH2
+            ; try contradiction.
+            apply nnrs_imp_stmt_eval_domain_stack in eqq.
+            apply nnrs_imp_stmt_eval_domain_stack in eqq4.
+            fuse_tt.
+            rewrite lookup_app.
+            rewrite lookup_nin_none; [|  unfold domain in *; congruence].
+            simpl.
+            destruct (equiv_dec s s); [| congruence].
+            exists o0.
+            rewrite update_app_nin; [|  unfold domain in *; congruence].
+            simpl.
+            destruct (equiv_dec s s); [| congruence].
+            specialize (HH1 ((s,o1)::x3) o2 x4); simpl in HH1.
+            cut_to HH1; [| unfold domain in *; congruence | trivial].
+            specialize (HH2 ((s,o)::x1) o0 x2); simpl in HH2.
+            cut_to HH2; [| unfold domain in *; congruence | trivial].
+            destruct HH1; subst.
+            fuse_tt.
+            split; trivial.
+          * assert (σ_bt_cons : pd_bindings_type ((v1, Some d0) :: σ) ((v1, τr) :: Γ)).
+            {
+              econstructor; simpl; trivial.
+              split; trivial; intros.
+              invcs H; trivial.
+            } 
+            specialize (IHs2 _ ((v1, Some d0)::σ) d eqq2 ((v1, τr) :: Γ) σ_bt_cons τ).
+            cut_to IHs2; simpl; trivial; try solve [match_destr; congruence].
+            specialize (IHs2 _ ft).
+            simpl in IHs2.
+            unfold var in *.
+            destruct (equiv_dec v v1); try congruence.
+            unfold lift2P in *.
+            do 2 match_option_in IHs2
+            ; try contradiction.
+            generalize (nnrs_imp_stmt_eval_domain_stack eqq)
+            ; generalize (nnrs_imp_stmt_eval_domain_stack eqq3)
+            ; intros.
+            fuse_tt.
+            destruct (equiv_dec v s); [congruence| ].
+            match_option_in IHs2.
+            destruct IHs2 as [dd' [HH1 HH2]].
+            invcs HH1.
+            exists dd'; split; trivial. 
+    Qed.
 
   End eval.
   
@@ -678,35 +678,35 @@ Section TNNRSimpUnflatten.
           invcs H2; rtype_equalizer; subst.
           destruct d; try discriminate.
           destruct l; try discriminate.
-            invcs H1.
-            econstructor.
-            rewrite <- H.
-            econstructor; trivial.
-        - Case "NNRSimpBinop"%string.
-          destruct b; try discriminate.
-          apply some_lift2 in eqq.
-          destruct eqq as [?[? eqq1[eqq2 ?]]]; subst.
-          invcs typ.
-          invcs H3.
-          apply Coll_right_inv in H; subst.
-          econstructor; eauto.
+          invcs H1.
           econstructor.
-        - Case "NNRSimpUnop"%string.
-          destruct u; try discriminate.
-          destruct e; try discriminate.
-          + destruct d; try discriminate.
-            invcs typ.
-            invcs H2.
-            apply Coll_right_inv in H; subst.
-            invcs eqq; trivial.
-          + destruct u; try discriminate.
-            invcs eqq.
-            invcs typ.
-            invcs H2.
-            apply Coll_right_inv in H; subst.
-            trivial.
+          rewrite <- H.
+          econstructor; trivial.
+      - Case "NNRSimpBinop"%string.
+        destruct b; try discriminate.
+        apply some_lift2 in eqq.
+        destruct eqq as [?[? eqq1[eqq2 ?]]]; subst.
+        invcs typ.
+        invcs H3.
+        apply Coll_right_inv in H; subst.
+        econstructor; eauto.
+        econstructor.
+      - Case "NNRSimpUnop"%string.
+        destruct u; try discriminate.
+        destruct e; try discriminate.
+        + destruct d; try discriminate.
+          invcs typ.
+          invcs H2.
+          apply Coll_right_inv in H; subst.
+          invcs eqq; trivial.
+        + destruct u; try discriminate.
+          invcs eqq.
+          invcs typ.
+          invcs H2.
+          apply Coll_right_inv in H; subst.
+          trivial.
     Qed.
-          
+    
     Lemma nnrs_imp_expr_unflatten_read_type e e' v :
       nnrs_imp_expr_unflatten_read e v = Some e' ->
       forall {Γc Γ τo},
@@ -717,59 +717,59 @@ Section TNNRSimpUnflatten.
     Proof.
       revert e'.
       nnrs_imp_expr_cases (induction e) Case
-        ; simpl ; intros e' eqq Γc Γ τo typ τ inn.
-        - Case "NNRSimpGetConstant"%string.
-          invcs eqq.
-          invcs typ.
-          econstructor; trivial.
-        - Case "NNRSimpVar"%string.
-          match_destr_in eqq.
-          invcs eqq; simpl.
-          invcs typ.
+      ; simpl ; intros e' eqq Γc Γ τo typ τ inn.
+      - Case "NNRSimpGetConstant"%string.
+        invcs eqq.
+        invcs typ.
+        econstructor; trivial.
+      - Case "NNRSimpVar"%string.
+        match_destr_in eqq.
+        invcs eqq; simpl.
+        invcs typ.
+        econstructor.
+        rewrite lookup_update_neq; trivial.
+        eauto.
+      - Case "NNRSimpConst"%string.
+        invcs eqq; simpl; trivial.
+        invcs typ.
+        econstructor; trivial.
+      - Case "NNRSimpBinop"%string.
+        apply some_lift2 in eqq.
+        destruct eqq as [?[? eqq1[eqq2 ?]]]; subst.
+        invcs typ.
+        econstructor; eauto.
+      - Case "NNRSimpUnop"%string.
+        invcs typ.
+        destruct u
+        ; try solve [apply some_lift in eqq
+                     ; destruct eqq as [eqq1 eqq2]
+                     ; subst; simpl
+                     ; econstructor; eauto].
+        destruct e
+        ; try solve [apply some_lift in eqq
+                     ; destruct eqq as [eqq1 eqq2]
+                     ; subst; simpl
+                     ; econstructor; eauto].
+        invcs H2.
+        invcs H4.
+        match_destr_in eqq.
+        + invcs eqq; simpl.
+          rewrite e in *.
+          unfold var in *.
+          rewrite inn in H1; invcs H1; rtype_equalizer.
+          apply Coll_right_inv in H0; subst.
           econstructor.
-          rewrite lookup_update_neq; trivial.
-          eauto.
-        - Case "NNRSimpConst"%string.
-          invcs eqq; simpl; trivial.
-          invcs typ.
-          econstructor; trivial.
-        - Case "NNRSimpBinop"%string.
-          apply some_lift2 in eqq.
-          destruct eqq as [?[? eqq1[eqq2 ?]]]; subst.
-          invcs typ.
-          econstructor; eauto.
-        - Case "NNRSimpUnop"%string.
-          invcs typ.
-          destruct u
-          ; try solve [apply some_lift in eqq
-          ; destruct eqq as [eqq1 eqq2]
-          ; subst; simpl
-          ; econstructor; eauto].
-          destruct e
-          ; try solve [apply some_lift in eqq
-                       ; destruct eqq as [eqq1 eqq2]
-                       ; subst; simpl
-                       ; econstructor; eauto].
-          invcs H2.
-          invcs H4.
-          match_destr_in eqq.
-          + invcs eqq; simpl.
-            rewrite e in *.
-            unfold var in *.
-            rewrite inn in H1; invcs H1; rtype_equalizer.
-            apply Coll_right_inv in H0; subst.
-            econstructor.
-            rewrite lookup_update_eq_in; try congruence.
-            apply lookup_in_domain in inn; trivial.
-          + invcs eqq; simpl.
-            econstructor; econstructor.
-            rewrite lookup_update_neq; eauto.
-        - Case "NNRSimpGroupBy"%string.
-          apply some_lift in eqq.
-          destruct eqq as [??]; subst; simpl.
-          invcs typ.
-          econstructor; trivial.
-          eauto.
+          rewrite lookup_update_eq_in; try congruence.
+          apply lookup_in_domain in inn; trivial.
+        + invcs eqq; simpl.
+          econstructor; econstructor.
+          rewrite lookup_update_neq; eauto.
+      - Case "NNRSimpGroupBy"%string.
+        apply some_lift in eqq.
+        destruct eqq as [??]; subst; simpl.
+        invcs typ.
+        econstructor; trivial.
+        eauto.
     Qed.
 
     Lemma nnrs_imp_expr_unflatten_write_type e e' v :
@@ -784,50 +784,50 @@ Section TNNRSimpUnflatten.
       nnrs_imp_expr_cases (induction e) Case
       ; simpl ; intros e' eqq Γc Γ τo typ τ inn
       ; try discriminate.
-        - Case "NNRSimpVar"%string.
-          match_destr_in eqq.
-          rewrite e in *; clear v0 e.
-          invcs eqq; simpl.
-          invcs typ.
-          rewrite inn in H1.
+      - Case "NNRSimpVar"%string.
+        match_destr_in eqq.
+        rewrite e in *; clear v0 e.
+        invcs eqq; simpl.
+        invcs typ.
+        rewrite inn in H1.
+        invcs H1.
+        apply Coll_right_inv in H0; subst.
+        econstructor.
+        rewrite lookup_update_eq_in; eauto.
+        apply lookup_in_domain in inn; trivial.
+      - Case "NNRSimpConst"%string.
+        invcs typ.
+        destruct d; simpl; try discriminate.
+        destruct l; simpl; try discriminate.
+        + invcs eqq.
+          econstructor.
+          repeat econstructor.
+        + destruct d; simpl; try discriminate.
+          destruct l; simpl; try discriminate.
+          invcs eqq.
+          econstructor.
+          simpl in H1.
           invcs H1.
           apply Coll_right_inv in H0; subst.
-          econstructor.
-          rewrite lookup_update_eq_in; eauto.
-          apply lookup_in_domain in inn; trivial.
-        - Case "NNRSimpConst"%string.
-          invcs typ.
-          destruct d; simpl; try discriminate.
-          destruct l; simpl; try discriminate.
-          + invcs eqq.
-            econstructor.
-            repeat econstructor.
-          + destruct d; simpl; try discriminate.
-             destruct l; simpl; try discriminate.
-             invcs eqq.
-             econstructor.
-             simpl in H1.
-             invcs H1.
-             apply Coll_right_inv in H0; subst.
-             invcs H2; trivial.
-        - Case "NNRSimpBinop"%string.
-          destruct b; try discriminate.
-          apply some_lift2 in eqq.
-          destruct eqq as [?[? eqq1[eqq2 ?]]]; subst.
-          invcs typ.
-          invcs H3.
-          apply Coll_right_inv in H; subst.
-          econstructor; eauto.
-          econstructor.
-        - Case "NNRSimpUnop"%string.
-          invcs typ.
-          destruct u; try discriminate.
-          match_destr_in eqq.
-          invcs eqq.
-          invcs H2.
-          apply Coll_right_inv in H; subst.
-          apply (nnrs_imp_expr_type_update_first_irrelevant Γc nil)
-          ; simpl; tauto.
+          invcs H2; trivial.
+      - Case "NNRSimpBinop"%string.
+        destruct b; try discriminate.
+        apply some_lift2 in eqq.
+        destruct eqq as [?[? eqq1[eqq2 ?]]]; subst.
+        invcs typ.
+        invcs H3.
+        apply Coll_right_inv in H; subst.
+        econstructor; eauto.
+        econstructor.
+      - Case "NNRSimpUnop"%string.
+        invcs typ.
+        destruct u; try discriminate.
+        match_destr_in eqq.
+        invcs eqq.
+        invcs H2.
+        apply Coll_right_inv in H; subst.
+        apply (nnrs_imp_expr_type_update_first_irrelevant Γc nil)
+        ; simpl; tauto.
     Qed.
 
     Lemma nnrs_imp_stmt_unflatten_type s s' v :
@@ -870,8 +870,8 @@ Section TNNRSimpUnflatten.
         destruct eqq as [?[? eqq1[eqq2 ?]]]; subst.
         invcs typ; simpl in *.
         + apply some_lift in eqq1.
-           destruct eqq1 as [? eqq1 ?]; subst; simpl.
-           econstructor.
+          destruct eqq1 as [? eqq1 ?]; subst; simpl.
+          econstructor.
           * eapply nnrs_imp_expr_unflatten_read_type in eqq1; eauto.
           * { match_destr_in eqq2; unfold equiv, complement in *.
               - invcs eqq2.
@@ -888,7 +888,7 @@ Section TNNRSimpUnflatten.
           * invcs eqq2.
             econstructor; trivial.
             apply (nnrs_imp_stmt_type_update_first_irrelevant Γc ((v, τ0) :: nil))
-                ; simpl; tauto.
+            ; simpl; tauto.
           * { econstructor.
               - rewrite <- (nnrs_imp_stmt_unflatten_var_usage eqq2); trivial.
               - specialize (IHs _ eqq2 _ _ H4).
@@ -974,24 +974,24 @@ Section TNNRSimpUnflatten.
         destruct inn1 as [inn1|inn1]; eauto.
       - Case "NNRSimpUnop"%string.
         invcs typ.
-          destruct u
-          ; try solve [apply some_lift in eqq
+        destruct u
+        ; try solve [apply some_lift in eqq
                      ; destruct eqq as [eqq1 eqq2]
                      ; subst; simpl
                      ; invcs H2; eauto].
-          invcs H2.
-          destruct e
-          ; try solve [apply some_lift in eqq
+        invcs H2.
+        destruct e
+        ; try solve [apply some_lift in eqq
                      ; destruct eqq as [eqq1 eqq2]
                      ; subst; simpl; eauto].
-          simpl in inn1.
-          match_destr_in eqq; [ | intuition congruence].
-          invcs eqq.
-          invcs H4.
-          intuition; subst.
-          rewrite H1 in inn2.
-          invcs inn2.
-          eauto.
+        simpl in inn1.
+        match_destr_in eqq; [ | intuition congruence].
+        invcs eqq.
+        invcs H4.
+        intuition; subst.
+        rewrite H1 in inn2.
+        invcs inn2.
+        eauto.
       - Case "NNRSimpGroupBy"%string.
         apply some_lift in eqq.
         destruct eqq as [? eqq ?].
@@ -1083,8 +1083,8 @@ Section TNNRSimpUnflatten.
             eapply IHs1; eauto.
             simpl; match_destr; congruence.
         + match_destr_in eqq_ro.
-            eapply IHs2; eauto.
-            simpl; match_destr; congruence.
+          eapply IHs2; eauto.
+          simpl; match_destr; congruence.
     Qed.
 
   End type_enrich.
@@ -1092,24 +1092,24 @@ Section TNNRSimpUnflatten.
   Section unflatten_safe.
 
     Lemma nnrs_imp_stmt_unflatten_safe_eval s s' v σc σ d :
-        nnrs_imp_stmt_unflatten_safe s v = Some s' ->
-        forall Γc,
-          bindings_type σc Γc ->
-          forall Γ,
-            pd_bindings_type σ Γ ->
-            forall τ,
-              lookup equiv_dec σ v = Some d ->
-              lookup equiv_dec Γ v = Some τ ->
-              [ Γc ; Γ  ⊢ s ] ->
-              forall d',
-                lift2P flattens_to d d' ->
+      nnrs_imp_stmt_unflatten_safe s v = Some s' ->
+      forall Γc,
+        bindings_type σc Γc ->
+        forall Γ,
+          pd_bindings_type σ Γ ->
+          forall τ,
+            lookup equiv_dec σ v = Some d ->
+            lookup equiv_dec Γ v = Some τ ->
+            [ Γc ; Γ  ⊢ s ] ->
+            forall d',
+              lift2P flattens_to d d' ->
               lift2P
                 (fun σ₁' σ₂' =>
                    match lookup equiv_dec σ₁' v with
                    | Some dd => 
                      exists dd',
-                       σ₂' = update_first equiv_dec σ₁' v dd'
-                       /\ lift2P flattens_to dd dd'
+                     σ₂' = update_first equiv_dec σ₁' v dd'
+                     /\ lift2P flattens_to dd dd'
                    | None => False
                    end
                 )
@@ -1131,9 +1131,9 @@ Section TNNRSimpUnflatten.
         [ Γc ; Γ  ⊢ s]  ->
         forall τ,
           lookup equiv_dec Γ v = Some τ ->
-        exists τ',
-          [ Γc ; (update_first equiv_dec Γ v (Coll τ'))   ⊢ s']
-          /\  τ = Coll (Coll τ').
+          exists τ',
+            [ Γc ; (update_first equiv_dec Γ v (Coll τ'))   ⊢ s']
+            /\  τ = Coll (Coll τ').
     Proof.
       unfold nnrs_imp_stmt_unflatten_safe.
       intros eqq1 Γc Γ typ τ inn.
@@ -1145,9 +1145,9 @@ Section TNNRSimpUnflatten.
     Qed.
 
     Lemma nnrs_imp_stmt_unflatten_safe_var_usage {s s' v}:
-        nnrs_imp_stmt_unflatten_safe s v = Some s' ->
-        forall v',
-          nnrs_imp_stmt_var_usage s v' = nnrs_imp_stmt_var_usage s' v'.
+      nnrs_imp_stmt_unflatten_safe s v = Some s' ->
+      forall v',
+        nnrs_imp_stmt_var_usage s v' = nnrs_imp_stmt_var_usage s' v'.
     Proof.
       unfold nnrs_imp_stmt_unflatten_safe.
       intros eqq1; intros.
@@ -1155,7 +1155,16 @@ Section TNNRSimpUnflatten.
       eapply nnrs_imp_stmt_unflatten_var_usage; eauto.
     Qed.
 
-  End unflatten_safe.
+    Lemma nnrs_imp_stmt_unflatten_safe_var_usage_sub {s x s'} :
+      nnrs_imp_stmt_unflatten_safe s x = Some s' ->
+      stmt_var_usage_sub s s'.
+    Proof.
+      intros eqq1 v.
+      eapply nnrs_imp_stmt_unflatten_safe_var_usage in eqq1.
+      rewrite eqq1.
+      reflexivity.
+    Qed.
 
+  End unflatten_safe.
   
 End TNNRSimpUnflatten.
